Blocks.v
@@ -67,40 +67,12 @@ Record BlockInfo (blockType1 blockType2 opType1 opType2 : Set) := {
 
 Variable binfo : BlockInfo blockType1 blockType2 opType1 opType2.
 
-Definition BoundedRange (pos : nat) :=
-  { r : RangeSig | pos <= NE_head (ups r.1) }.
-
-Definition transportBoundedRange {base : nat} `(Hlt : base < prev)
-  (x : BoundedRange prev) : BoundedRange base.
-  case: x => [r H].
-  apply: exist.
-  apply: r.
-  exact/(leq_trans _ H)/ltnW.
-Defined.
-
-Definition BoundedInterval (pos : nat) :=
-  { i : IntervalSig | pos <= rbeg (NE_head (rds i.1)).1 }.
-
-Definition transportBoundedInterval {base : nat} `(Hlt : base < prev)
-  (x : BoundedInterval prev) : BoundedInterval base.
-  case: x => [i H].
-  apply: exist.
-  apply: i.
-  exact/(leq_trans _ H)/ltnW.
-Defined.
-
 (* jww (2015-01-12): Some of the things described by Wimmer in the section on
    dealing with computing of intervals have yet to be done:
 
    - Loop handling (reordering blocks to optimize allocation)
    - Extending of ranges for input/output variables
 *)
-
-Record BuildState := {
-  bsPos  : nat;
-  bsVars : seq (option (BoundedRange bsPos.*2.+1));
-  bsRegs : Vec (option (BoundedInterval bsPos.*2.+1)) maxReg
-}.
 
 Definition foldOps {a} (f : a -> opType1 -> a) (z : a) :
   seq blockType1 -> a :=
@@ -112,104 +84,6 @@ Definition foldOpsRev {a} (f : a -> opType1 -> a) (z : a)
   (blocks : seq blockType1) : a :=
   foldl (fun bacc blk => foldl f bacc (rev (blockOps binfo blk)))
         z (rev blocks).
-
-Lemma inner_addn1: forall n, n.*2.+1 < (n.+1).*2.+1.
-Proof. by move=> n; rewrite doubleS. Qed.
-
-(* For each virtual variable references, add a use position to a [Range]
-   corresponding to that variable.  These ranges are concatenated together and
-   will form a single [Interval] at the end.  This is different from how
-   Wimmer builds them up, and is more simplistic, but is sufficient for now.
-
-   jww (2015-01-30): The more efficient solution would be to implement the
-   algorithm from his paper. *)
-Definition createRangeForVars (pos : nat)
-  (vars : seq (option (BoundedRange (pos.+1).*2.+1)))
-  (varRefs : seq varType) : seq (option (BoundedRange pos.*2.+1)).
-Proof.
-  have vars' := vars.
-  move/(map (option_map (transportBoundedRange
-                           (inner_addn1 pos)))) in vars'.
-  apply: foldl _ vars' varRefs => vars' v.
-
-  (* jww (2015-01-30): The [regReq] field is presently not being used. *)
-  set upos := {| uloc   := pos.*2.+1
-               ; regReq := regRequired vinfo v |}.
-  have Hodd : odd upos by rewrite /= odd_double.
-
-  apply: (set_nth None vars' (varId vinfo v) _).
-  apply: Some _.
-  case: (nth None vars (varId vinfo v)) => [[r /= Hlt]|];
-    last exact: exist _ (exist _ _ (R_Sing Hodd)) _.
-
-  apply: exist _ (exist _ _ (R_Cons Hodd r.2 _)) _ => //=.
-  rewrite doubleS in Hlt.
-  exact/ltnW.
-Defined.
-
-(* For each register that is explicitly referenced by the operation, build up
-   a [Interval] which excludes this register from use, but only at specific
-   one-position wide ranges. *)
-Definition createIntervalForRegs (pos : nat)
-  (regs : Vec (option (BoundedInterval (pos.+1).*2.+1)) maxReg)
-  (regRefs : seq PhysReg) :
-  Vec (option (BoundedInterval pos.*2.+1)) maxReg.
-Proof.
-  have regs' := regs.
-  move/(vmap (option_map (transportBoundedInterval
-                            (inner_addn1 pos)))) in regs'.
-  apply: foldl _ regs' regRefs => regs' reg.
-
-  set upos := {| uloc   := pos.*2.+1
-               ; regReq := true |}.
-  have Hodd : odd upos by rewrite /= odd_double.
-
-  set r := exist _ _ (R_Sing Hodd).
-  apply: (vreplace regs' reg _).
-  apply: Some _.
-  case: (vnth regs reg) => [[[d i] /= Hlt]|];
-    last exact: exist _ (exist _ _ (I_Sing 0 Whole r.2)) _.
-
-  case: d => [iv ib ie ik rds] in i Hlt *.
-  rewrite /= in Hlt.
-  have Hrds: rend r.1 < rbeg (NE_head rds).1.
-    rewrite /r /=.
-    by rewrite doubleS in Hlt.
-  move: (Interval_exact_beg i)
-        (Interval_exact_end i) => /= Hbeg Hend.
-  move: Hbeg Hend i => -> -> i.
-  exact: exist _ (exist _ _ (I_Cons i Hrds)) _ => //=.
-Defined.
-
-Definition processOperations (blocks : seq blockType1) : BuildState.
-  have := foldOps (fun x op => let: (n, m) := x in
-    (n.+1, foldl (fun m v => maxn m (varId vinfo v))
-                 m (fst (opRefs oinfo op))))
-    (0, 0) blocks.
-  move=> [opCount highestVar].
-  pose z := {| bsPos  := opCount
-             ; bsVars := nseq highestVar.+1 None
-             ; bsRegs := vconst None |}.
-  apply: (foldOpsRev _ z blocks).
-  case=> [pos vars regs] op.
-  case: pos => [|pos] in vars regs *.
-    exact {| bsPos  := 0
-           ; bsVars := vars
-           ; bsRegs := regs |}.
-  move: (opRefs oinfo op) => [varRefs regRefs].
-  apply: {| bsPos  := pos |}.
-    exact: createRangeForVars.
-
-  (* If the operation is a function call, assuming it makes use of every
-     register.
-
-     jww (2015-01-30): This needs to be improved to consider the calling
-     convention of the operation. *)
-  have regRefs' := if opKind oinfo op is IsCall
-                   then enum 'I_maxReg else regRefs.
-  clear regRefs.
-  exact: createIntervalForRegs.
-Defined.
 
 (* jww (2014-11-19): Note that we are currently not computing the block order
    in any intelligent way. This is covered in quite some depth in Christian
@@ -228,13 +102,6 @@ Definition computeBlockOrder (blocks : seq blockType1) : seq blockType1 :=
    data at the very end. *)
 Definition numberOperations (blocks : seq blockType1) : seq blockType1 :=
   blocks.
-  (* let f n op := *)
-  (*   (n.+2, {| opId    := n *)
-  (*           ; opMeta  := opMeta op *)
-  (*           ; opKind  := opKind op *)
-  (*           ; varRefs := varRefs op *)
-  (*           ; regRefs := regRefs op |}) in *)
-  (* imodify SSError (@snd _ _ \o mapAccumLOps f 1). *)
 
 Inductive IntMap (a : Type) :=
   | emptyIntMap
@@ -406,6 +273,282 @@ Definition computeGlobalLiveSets (blocks : seq blockType1)
          |} liveSets1
     end.
 
+(* For each virtual variable references, add a use position to a [Range]
+   corresponding to that variable.  These ranges are concatenated together and
+   will form a single [Interval] at the end.  This is different from how
+   Wimmer builds them up, and is more simplistic, but is sufficient for now.
+
+   jww (2015-01-30): The more efficient solution would be to implement the
+   algorithm from his paper. *)
+Definition createRangeForVars (pos : nat)
+  (vars : seq (option (BoundedRange (pos.+1).*2.+1)))
+  (varRefs : seq varType) : seq (option (BoundedRange pos.*2.+1)).
+Proof.
+  have vars' := vars.
+  move/(map (option_map (transportBoundedRange
+                           (inner_addn1 pos)))) in vars'.
+  apply: foldl _ vars' varRefs => vars' v.
+
+  (* jww (2015-01-30): The [regReq] field is presently not being used. *)
+  set upos := {| uloc   := pos.*2.+1
+               ; regReq := regRequired vinfo v |}.
+  have Hodd : odd upos by rewrite /= odd_double.
+
+  apply: (set_nth None vars' (varId vinfo v) _).
+  apply: Some _.
+  case: (nth None vars (varId vinfo v)) => [[r /= Hlt]|];
+    last exact: exist _ (exist _ _ (R_Sing Hodd)) _.
+
+  apply: exist _ (exist _ _ (R_Cons Hodd r.2 _)) _ => //=.
+  rewrite doubleS in Hlt.
+  exact/ltnW.
+Defined.
+
+(* For each register that is explicitly referenced by the operation, build up
+   a [Interval] which excludes this register from use, but only at specific
+   one-position wide ranges. *)
+Definition setIntervalsForRegs (pos : nat)
+  (regs : Vec (option (BoundedInterval (pos.+1).*2.+1)) maxReg)
+  (regRefs : seq PhysReg) :
+  Vec (option (BoundedInterval pos.*2.+1)) maxReg.
+Proof.
+  have regs' := regs.
+  move/(vmap (option_map (transportBoundedInterval
+                            (inner_addn1 pos)))) in regs'.
+  apply: foldl _ regs' regRefs => regs' reg.
+
+  set upos := {| uloc   := pos.*2.+1
+               ; regReq := true |}.
+  have Hodd : odd upos by rewrite /= odd_double.
+
+  set r := exist _ _ (R_Sing Hodd).
+  apply: (vreplace regs' reg _).
+  apply: Some _.
+  case: (vnth regs reg) => [[[d i] /= Hlt]|];
+    last exact: exist _ (exist _ _ (I_Sing 0 Whole r.2)) _.
+
+  case: d => [iv ib ie ik rds] in i Hlt *.
+  rewrite /= in Hlt.
+  have Hrds: rend r.1 < rbeg (NE_head rds).1.
+    rewrite /r /=.
+    by rewrite doubleS in Hlt.
+  move: (Interval_exact_beg i)
+        (Interval_exact_end i) => /= Hbeg Hend.
+  move: Hbeg Hend i => -> -> i.
+  exact: exist _ (exist _ _ (I_Cons i Hrds)) _ => //=.
+Defined.
+
+Record BuildState (pos : nat) := {
+  bsVars : seq (option (SortedBoundedRanges pos.*2.+1));
+  bsRegs : Vec (option (BoundedInterval pos.*2.+1)) maxReg
+}.
+
+Definition transportSortedBoundedRanges {base : nat} `(Hlt : base < prev)
+  (sr : SortedBoundedRanges prev) : SortedBoundedRanges base.
+Proof.
+  case: sr => [rs Hsort].
+  exists (NE_map (transportBoundedRange Hlt) rs).
+  elim: rs => [r|r rs IHrs] /= in Hsort *.
+    by constructor.
+  constructor; inversion Hsort; subst.
+    exact: IHrs.
+  exact: NE_Forall_transport.
+Defined.
+
+Definition reduceOp {pos} (op : opType1) (block : blockType1)
+  (bs : BuildState pos.+1) : BuildState pos :=
+  let: (varRefs, regRefs) := opRefs oinfo op in
+
+  (* If the operation is a function call, assuming it makes use of every
+     register.
+     jww (2015-01-30): This needs to be improved to consider the calling
+     convention of the operation. *)
+  let regRefs' := if opKind oinfo op is IsCall
+                  then enum 'I_maxReg
+                  else regRefs in
+  {| bsVars := map (option_map (transportSortedBoundedRanges (ltnSSn _)))
+                   (bsVars bs)
+   ; bsRegs := setIntervalsForRegs (bsRegs bs) regRefs' |}.
+
+Definition reduceBlock {pos} (block : blockType1) (liveOut : IntSet)
+  (bs : BuildState (pos + size (blockOps binfo block))) : BuildState pos.
+  elim: (blockOps binfo block) => [|o os IHos] /= in bs *.
+    by rewrite addn0 in bs.
+  rewrite addnS in bs.
+  exact: (IHos (reduceOp o block bs)).
+Defined.
+
+Definition reduceBlocks (blocks : seq blockType1)
+  (liveSets : IntMap BlockLiveSets) : BuildState 0 :=
+  let: highestVar :=
+      foldOps (fun n op =>
+        foldl (fun m v => maxn m (varId vinfo v)) n
+              (fst (opRefs oinfo op)))
+        0 blocks in
+  let fix go b bs pos : BuildState pos :=
+      let bid  := blockId binfo b in
+      let outs := if IntMap_lookup bid liveSets isn't Some ls
+                  then emptyIntSet
+                  else blockLiveOut ls in
+      reduceBlock outs $ match bs with
+        | nil => {| bsVars := nseq highestVar.+1 None
+                  ; bsRegs := vconst None |}
+        | cons b' bs' => go b' bs' (pos + size (blockOps binfo b))
+        end in
+  match blocks with
+  | nil => {| bsVars := nseq highestVar.+1 None
+            ; bsRegs := vconst None |}
+  | cons x xs => go x xs 0
+  end.
+
+Definition buildIntervals (blocks : seq blockType1)
+  (liveSets : IntMap BlockLiveSets) : ScanStateSig InUse :=
+  (* for each block b in blocks in reverse order do
+       int block_from = b.first_op.id
+       int block_to = b.last_op.id + 2
+
+       for each operand opr in b.live_out do
+         intervals[opr].add_range(block_from, block_to)
+       end for
+
+       for each operation op in b.operations in reverse order do
+         visitor.visit(op)
+
+         if visitor.has_call then
+           for each physical register reg do
+             intervals[reg].add_range(op.id, op.id + 1)
+           end for
+         end if
+
+         for each virtual or physical register opr in visitor.output_oprs do
+           intervals[opr].first_range.from = op.id
+           intervals[opr].add_use_pos(op.id, use_kind_for(op, opr))
+         end for
+
+         for each virtual or physical register opr in visitor.temp_oprs do
+           intervals[opr].add_range(op.id, op.id + 1)
+           intervals[opr].add_use_pos(op.id, use_kind_for(op, opr))
+         end for
+
+         for each virtual or physical register opr in visitor.input_oprs do
+           intervals[opr].add_range(block_from, op.id)
+           intervals[opr].add_use_pos(op.id, use_kind_for(op, opr))
+         end for
+       end for
+     end for *)
+  let mkint
+        (vid : VarId)
+        (ss  : ScanStateSig Pending)
+        (pos : nat)
+        (mrs : option (SortedBoundedRanges pos.*2.+1))
+        (f   : forall sd, ScanState Pending sd
+                 -> forall d, Interval d -> ScanStateSig Pending) :=
+      if mrs is Some rs
+      then f _ ss.2 _ (packInterval (Interval_fromRanges vid rs)).2
+      else ss in
+
+  let handleVar pos vid ss mrs :=
+      mkint vid ss pos mrs $ fun _ st _ i =>
+        packScanState (ScanState_newUnhandled st i I) in
+
+  (fun (bs : BuildState 0) =>
+     let s0 := ScanState_nil in
+     let f mx := if mx is Some x then Some x.1 else None in
+     let regs := vmap f (bsRegs bs) in
+     let s1 := ScanState_setFixedIntervals s0 regs in
+     let s2 := packScanState s1 in
+     let s3 := foldl_with_index (handleVar 0) s2 (bsVars bs) in
+     let s4 := ScanState_finalize s3.2 in
+     packScanState s4)
+  (reduceBlocks blocks liveSets).
+
+(*
+  have [opCount highestVar] :=
+      foldOps (fun x op => let: (n, m) := x in
+        (n.+1, foldl (fun m v => maxn m (varId vinfo v))
+                     m (fst (opRefs oinfo op))))
+        (0, 0) blocks.
+  have :=
+      {| bsPos  := opCount
+       ; bsVars := nseq highestVar.+1 [::]
+       ; bsRegs := vconst None |}.
+  case=> [pos vars regs].
+  case: pos => [|pos] in vars regs *.
+    exact {| bsPos  := 0
+           ; bsVars := vars
+           ; bsRegs := regs |}.
+
+  apply: {| bsPos := pos |}.
+  move: (opRefs oinfo op) => [varRefs regRefs].
+    exact: createRangeForVars.
+
+  (* If the operation is a function call, assuming it makes use of every
+     register.
+
+     jww (2015-01-30): This needs to be improved to consider the calling
+     convention of the operation. *)
+  have regRefs' := if opKind oinfo op is IsCall
+                   then enum 'I_maxReg else regRefs.
+  clear regRefs.
+  exact: createIntervalForRegs.
+Defined.
+
+  let fix go pos (bst : BuildState pos) bs :=
+    if bs isn't b :: bs then bst else
+    let bid  := blockId binfo b in
+    let outs := if IntMap_lookup bid liveSets isn't Some ls
+                then emptyIntSet
+                else blockLiveOut ls in
+    match pos with
+    | 0 => bst
+    | S pos' =>
+      let Heqe : pos'.+1 = pos := undefined in
+      let bst' :=
+        forFold bst (rev (blockOps binfo b)) $ fun bst' op =>
+          let: (varRefs, regRefs) := opRefs oinfo op in
+
+          (* If the operation is a function call, assuming it makes use of every
+             register.
+             jww (2015-01-30): This needs to be improved to consider the calling
+             convention of the operation. *)
+          let regRefs' := if opKind oinfo op is IsCall
+                          then enum 'I_maxReg
+                          else regRefs in
+          let bsRegs' := @setIntervalsForRegs pos' (bsRegs bst') regRefs' in
+          {| bsVars := map (map (transportBoundedRange _)) (bsVars bst')
+           ; bsRegs := bsRegs' |} in
+      bst'
+    end in
+  go bst0 opCount (rev blocks).
+
+  forFold bst0 (rev blocks) $ fun bst1 b => match bsPos bst1 with
+    | 0 =>
+        {| bsPos  := 0
+         ; bsVars := map (map (transportBoundedRange _)) (bsVars bst1)
+         ; bsRegs := vmap (option_map (transportBoundedInterval _))
+                          (bsRegs bst1)
+         |}
+    | S pos =>
+      let bid  := blockId binfo b in
+      let outs := if IntMap_lookup bid liveSets isn't Some ls
+                  then emptyIntSet
+                  else blockLiveOut ls in
+      let bst4 :=
+        forFold bst1 (rev (blockOps binfo b)) $ fun bst2 op =>
+          let: (varRefs, regRefs) := opRefs oinfo op in
+
+          (* If the operation is a function call, assuming it makes use of every
+             register.
+             jww (2015-01-30): This needs to be improved to consider the calling
+             convention of the operation. *)
+          let regRefs' := if opKind oinfo op is IsCall
+                          then enum 'I_maxReg
+                          else regRefs in
+          let bst3 := @setIntervalsForRegs pos (bsRegs bst2) regRefs' in
+          bst3 in
+      bst4
+    end.
+
 Definition buildIntervals (blocks : seq blockType1) : ScanStateSig InUse :=
   let mkint (vid : VarId)
             (ss : ScanStateSig Pending)
@@ -434,6 +577,7 @@ Definition buildIntervals (blocks : seq blockType1) : ScanStateSig InUse :=
      let s4 := ScanState_finalize s3.2 in
      packScanState s4)
   (processOperations blocks).
+*)
 
 Definition checkIntervalBoundary `(st : ScanState InUse sd)
   key in_from from to mappings vid :=
